Updated bounded operators.

QHoare.thy
@@ -12,7 +12,7 @@ begin
 
 definition "apply U R = R U" for R :: \<open>'a update \<Rightarrow> 'mem update\<close>
 definition "ifthen R x = R (butterket x x)" for R :: \<open>'a update \<Rightarrow> 'mem update\<close>
-definition "program S = fold (o\<^sub>C\<^sub>L) S idOp" for S :: \<open>'mem update list\<close>
+definition "program S = fold (o\<^sub>C\<^sub>L) S id_cblinfun" for S :: \<open>'mem update list\<close>
 
 
 definition hoare :: \<open>'mem ell2 ccsubspace \<Rightarrow> ('mem ell2 \<Rightarrow>\<^sub>C\<^sub>L 'mem ell2) list \<Rightarrow> 'mem ell2 ccsubspace \<Rightarrow> bool\<close> where
@@ -21,16 +21,16 @@ definition hoare :: \<open>'mem ell2 ccsubspace \<Rightarrow> ('mem ell2 \<Right
 definition EQ :: "('a update \<Rightarrow> 'mem update) \<Rightarrow> 'a ell2 \<Rightarrow> 'mem ell2 ccsubspace" (infix "=\<^sub>q" 75) where
   "EQ R \<psi> = R (selfbutter \<psi>) *\<^sub>S \<top>"
 
-lemma program_skip[simp]: "program [] = idOp"
+lemma program_skip[simp]: "program [] = id_cblinfun"
   by (simp add: qhoare.program_def)
 
 lemma program_seq: "program (p1@p2) = program p2 o\<^sub>C\<^sub>L program p1"
   apply (induction p2 rule:rev_induct)
    apply (simp_all add: program_def)
-  by (meson assoc_left(1))
+  by (meson cblinfun_assoc_left(1))
 
 lemma hoare_seq[trans]: "hoare C p1 D \<Longrightarrow> hoare D p2 E \<Longrightarrow> hoare C (p1@p2) E"
-  by (auto simp: program_seq hoare_def times_applyOp)
+  by (auto simp: program_seq hoare_def)
 
 lemma hoare_weaken_left[trans]: \<open>A \<le> B \<Longrightarrow> hoare B p C \<Longrightarrow> hoare A p C\<close>
   unfolding hoare_def
@@ -41,22 +41,22 @@ lemma hoare_weaken_right[trans]: \<open>hoare A p B \<Longrightarrow> B \<le> C 
   by (meson in_mono less_eq_ccsubspace.rep_eq) 
 
 lemma hoare_skip: "C \<le> D \<Longrightarrow> hoare C [] D"
-  by (auto simp: program_def hoare_def times_applyOp in_mono less_eq_ccsubspace.rep_eq)
+  by (auto simp: program_def hoare_def in_mono less_eq_ccsubspace.rep_eq)
 
 lemma hoare_apply: 
   assumes "R U *\<^sub>S pre \<le> post"
   shows "hoare pre [apply U R] post"
   using assms 
   apply (auto simp: hoare_def program_def apply_def)
-  by (metis (no_types, lifting) applyOpSpace.rep_eq closure_subset imageI less_eq_ccsubspace.rep_eq subsetD)
+  by (metis (no_types, lifting) cblinfun_image.rep_eq closure_subset imageI less_eq_ccsubspace.rep_eq subsetD)
 
 lemma hoare_ifthen: 
   fixes R :: \<open>'a update \<Rightarrow> 'mem update\<close>
   assumes "R (selfbutter (ket x)) *\<^sub>S pre \<le> post"
   shows "hoare pre [ifthen R x] post"
   using assms 
-  apply (auto simp: hoare_def program_def ifthen_def butterfly_def')
-  by (metis (no_types, lifting) applyOpSpace.rep_eq closure_subset imageI less_eq_ccsubspace.rep_eq subsetD)
+  apply (auto simp: hoare_def program_def ifthen_def butterfly_def)
+  by (metis (no_types, lifting) cblinfun_image.rep_eq closure_subset imageI less_eq_ccsubspace.rep_eq subsetD)
 
 end
 
