Finite_Tensor_Product.thy
@@ -4,6 +4,8 @@ theory Finite_Tensor_Product
   imports Bounded_Operators.Complex_L2 Misc
 begin
 
+declare cblinfun.scaleC_right[simp]
+
 unbundle cblinfun_notation
 no_notation m_inv ("inv\<index> _" [81] 80)
 
@@ -63,10 +65,8 @@ proof -
     using S_def cindependent_ket by blast
   moreover have \<open>cspan S = UNIV\<close>
     using S_def cspan_ket_finite by blast
-  moreover have \<open>finite S\<close>
-    using S_def finite_class.finite_UNIV by blast
   ultimately have "cblinfun_extension_exists S \<phi>'"
-    by (rule cblinfun_extension_exists_finite)
+    by (rule cblinfun_extension_exists_finite_dim)
   then have "\<exists>P. \<forall>x\<in>S. P *\<^sub>V x = \<phi>' x"
     unfolding cblinfun_extension_exists_def by auto
   then have ex: \<open>\<exists>P. \<forall>a c. P *\<^sub>V ket (a,c) = \<phi> (a,c)\<close>
@@ -84,13 +84,13 @@ qed
 lemma tensor_op_ell2: "tensor_op A B *\<^sub>V tensor_ell2 \<psi> \<phi> = tensor_ell2 (A *\<^sub>V \<psi>) (B *\<^sub>V \<phi>)"
 proof -
   have 1: \<open>clinear (\<lambda>a. tensor_op A B *\<^sub>V tensor_ell2 a (ket b))\<close> for b
-    by (auto intro!: clinearI simp: tensor_ell2_add1 tensor_ell2_scaleC1 cblinfun_apply_add)
+    by (auto intro!: clinearI simp: tensor_ell2_add1 tensor_ell2_scaleC1 cblinfun.add_right)
   have 2: \<open>clinear (\<lambda>a. tensor_ell2 (A *\<^sub>V a) (B *\<^sub>V ket b))\<close> for b
-    by (auto intro!: clinearI simp: tensor_ell2_add1 tensor_ell2_scaleC1 cblinfun_apply_add)
+    by (auto intro!: clinearI simp: tensor_ell2_add1 tensor_ell2_scaleC1 cblinfun.add_right)
   have 3: \<open>clinear (\<lambda>a. tensor_op A B *\<^sub>V tensor_ell2 \<psi> a)\<close>
-    by (auto intro!: clinearI simp: tensor_ell2_add2 tensor_ell2_scaleC2 cblinfun_apply_add)
+    by (auto intro!: clinearI simp: tensor_ell2_add2 tensor_ell2_scaleC2 cblinfun.add_right)
   have 4: \<open>clinear (\<lambda>a. tensor_ell2 (A *\<^sub>V \<psi>) (B *\<^sub>V a))\<close>
-    by (auto intro!: clinearI simp: tensor_ell2_add2 tensor_ell2_scaleC2 cblinfun_apply_add)
+    by (auto intro!: clinearI simp: tensor_ell2_add2 tensor_ell2_scaleC2 cblinfun.add_right)
 
   have eq_ket_ket: \<open>tensor_op A B *\<^sub>V tensor_ell2 (ket a) (ket b) = tensor_ell2 (A *\<^sub>V ket a) (B *\<^sub>V ket b)\<close> for a b
     by (simp add: tensor_op_ket)
@@ -107,7 +107,7 @@ lemma comp_tensor_op: "(tensor_op a b) o\<^sub>C\<^sub>L (tensor_op c d) = tenso
   c :: "'a::finite ell2 \<Rightarrow>\<^sub>C\<^sub>L 'e ell2" and d :: "'b::finite ell2 \<Rightarrow>\<^sub>C\<^sub>L 'f ell2"
   apply (rule equal_ket)
   apply (rename_tac ij, case_tac ij, rename_tac i j, hypsubst_thin)
-  by (simp flip: tensor_ell2_ket add: tensor_op_ell2 times_applyOp)
+  by (simp flip: tensor_ell2_ket add: tensor_op_ell2 cblinfun_apply_cblinfun_compose)
 
 
 lemma tensor_op_cbilinear: \<open>cbilinear (tensor_op :: 'a::finite ell2 \<Rightarrow>\<^sub>C\<^sub>L 'b::finite ell2
@@ -116,16 +116,16 @@ proof -
   have \<open>clinear (\<lambda>b::'c ell2 \<Rightarrow>\<^sub>C\<^sub>L 'd ell2. tensor_op a b)\<close> for a :: \<open>'a ell2 \<Rightarrow>\<^sub>C\<^sub>L 'b ell2\<close>
     apply (rule clinearI)
      apply (rule equal_ket, rename_tac ij, case_tac ij, rename_tac i j, hypsubst_thin)
-     apply (simp flip: tensor_ell2_ket add: tensor_op_ell2 apply_cblinfun_distr_left tensor_ell2_add2)
+     apply (simp flip: tensor_ell2_ket add: tensor_op_ell2 cblinfun.add_left tensor_ell2_add2)
     apply (rule equal_ket, rename_tac ij, case_tac ij, rename_tac i j, hypsubst_thin)
-    by (simp flip: tensor_ell2_ket add: tensor_op_ell2 apply_cblinfun_distr_left tensor_ell2_scaleC2)
+    by (simp add: scaleC_cblinfun.rep_eq tensor_ell2_scaleC2 tensor_op_ket)
 
   moreover have \<open>clinear (\<lambda>a::'a::finite ell2 \<Rightarrow>\<^sub>C\<^sub>L 'b::finite ell2. tensor_op a b)\<close> for b :: \<open>'c ell2 \<Rightarrow>\<^sub>C\<^sub>L 'd ell2\<close>
     apply (rule clinearI)
      apply (rule equal_ket, rename_tac ij, case_tac ij, rename_tac i j, hypsubst_thin)
-     apply (simp flip: tensor_ell2_ket add: tensor_op_ell2 apply_cblinfun_distr_left tensor_ell2_add1)
+     apply (simp flip: tensor_ell2_ket add: tensor_op_ell2 cblinfun.add_left tensor_ell2_add1)
     apply (rule equal_ket, rename_tac ij, case_tac ij, rename_tac i j, hypsubst_thin)
-    by (simp flip: tensor_ell2_ket add: tensor_op_ell2 apply_cblinfun_distr_left tensor_ell2_scaleC1)
+    by (simp add: scaleC_cblinfun.rep_eq tensor_ell2_scaleC1 tensor_op_ket)
 
   ultimately show ?thesis
     unfolding cbilinear_def by auto
@@ -135,7 +135,7 @@ qed
 lemma tensor_butter: \<open>tensor_op (butterket i j) (butterket k l) = butterket (i,k) (j,l)\<close>
   for i :: "_" and j :: "_::finite" and k :: "_" and l :: "_::finite"
   apply (rule equal_ket, rename_tac x, case_tac x)
-  apply (auto simp flip: tensor_ell2_ket simp: times_applyOp tensor_op_ell2 butterfly_def')
+  apply (auto simp flip: tensor_ell2_ket simp: cblinfun_apply_cblinfun_compose tensor_op_ell2 butterfly_def)
   by (auto simp: tensor_ell2_scaleC1 tensor_ell2_scaleC2)
 
 lemma cspan_tensor_op: \<open>cspan {tensor_op (butterket i j) (butterket k l)| i (j::_::finite) k (l::_::finite). True} = UNIV\<close>
@@ -164,21 +164,28 @@ proof (rule ext, rule complex_vector.linear_eq_on_span[where f=F and g=G])
     using that by (auto simp: tensor_eq)
 qed
 
-lemma tensor_id[simp]: \<open>tensor_op idOp idOp = idOp\<close>
+lemma tensor_id[simp]: \<open>tensor_op id_cblinfun id_cblinfun = id_cblinfun\<close>
   apply (rule equal_ket, rename_tac x, case_tac x)
   by (simp flip: tensor_ell2_ket add: tensor_op_ell2)
 
 lemma tensor_op_adjoint: \<open>(tensor_op a b)* = tensor_op (a*) (b*)\<close>
   apply (rule cinner_ket_adjointI[symmetric])
   apply (auto simp flip: tensor_ell2_ket simp: tensor_op_ell2)
-  by (simp add: adjoint_I)
+  by (simp add: cinner_adj_left)
 
 lemma tensor_butterfly[simp]: "tensor_op (butterfly \<psi> \<psi>') (butterfly \<phi> \<phi>') = butterfly (tensor_ell2 \<psi> \<phi>) (tensor_ell2 \<psi>' \<phi>')"
   apply (rule equal_ket, rename_tac x, case_tac x)
-  by (simp flip: tensor_ell2_ket add: tensor_op_ell2 butterfly_def'
-      times_applyOp tensor_ell2_scaleC1 tensor_ell2_scaleC2)
+  by (simp flip: tensor_ell2_ket add: tensor_op_ell2 butterfly_def
+      cblinfun_apply_cblinfun_compose tensor_ell2_scaleC1 tensor_ell2_scaleC2)
 
+(* TODO move to BO library misc *)
+instance prod :: (CARD_1, CARD_1) CARD_1
+  apply intro_classes
+  by (simp add: CARD_1)
 
+(* TODO move to BO library *)
+instance cblinfun :: (\<open>{cfinite_dim,complex_normed_vector}\<close>, \<open>{cfinite_dim,complex_normed_vector}\<close>) cfinite_dim
+  sorry
 
 definition tensor_lift :: \<open>(('a1::finite ell2 \<Rightarrow>\<^sub>C\<^sub>L 'a2::finite ell2) \<Rightarrow> ('b1::finite ell2 \<Rightarrow>\<^sub>C\<^sub>L 'b2::finite ell2) \<Rightarrow> 'c)
                         \<Rightarrow> ((('a1\<times>'b1) ell2 \<Rightarrow>\<^sub>C\<^sub>L ('a2\<times>'b2) ell2) \<Rightarrow> 'c::complex_vector)\<close> where
@@ -201,11 +208,11 @@ proof -
     obtain i  j  k  l  where x: "x = (i,j,k,l)" by (meson prod_cases4) 
     obtain i' j' k' l' where y: "y = (i',j',k',l')" by (meson prod_cases4) 
     have 1: "bra (i,k) *\<^sub>V t4 x *\<^sub>V ket (j,l) = 1"
-      by (auto simp: t4_def x tensor_op_ell2 butterfly_def' times_applyOp ket_Kronecker_delta_eq
+      by (auto simp: t4_def x tensor_op_ell2 butterfly_def cblinfun_apply_cblinfun_compose ket_Kronecker_delta_eq
                simp flip: tensor_ell2_ket)
     assume \<open>x \<noteq> y\<close>
     then have 2: "bra (i,k) *\<^sub>V t4 y *\<^sub>V ket (j,l) = 0"
-      by (auto simp: t4_def x y tensor_op_ell2 butterfly_def' times_applyOp ket_Kronecker_delta_neq
+      by (auto simp: t4_def x y tensor_op_ell2 butterfly_def cblinfun_apply_cblinfun_compose ket_Kronecker_delta_neq
                simp flip: tensor_ell2_ket)
     from 1 2 that
     show False
@@ -221,7 +228,8 @@ proof -
     using image_iff by fastforce
 
   have "cblinfun_extension_exists (range t4) \<phi>"
-    apply (rule cblinfun_extension_exists_finite)
+    thm cblinfun_extension_exists_finite_dim[where \<phi>=\<phi>]
+    apply (rule cblinfun_extension_exists_finite_dim)
     apply auto unfolding * 
     using cindependent_tensor_op
     using cspan_tensor_op
@@ -240,12 +248,12 @@ proof -
     unfolding linfun_cspan
     using * apply (auto intro!: clinear_compose[unfolded o_def, where f=\<open>\<lambda>a. tensor_op a _\<close> and g=\<open>(*\<^sub>V) G\<close>])
      apply (metis cbilinear_def tensor_op_cbilinear)
-    apply (simp add: cblinfun_apply_add clinearI)
+    using bounded_clinear.axioms(1) cblinfun_apply apply blast
     using assms unfolding cbilinear_def by blast
   have G_F2: \<open>G *\<^sub>V tensor_op a b = F2 a b\<close> for a b
     apply (rule complex_vector.linear_eq_on_span[where g=\<open>F2 a\<close> and B=\<open>{butterket k l|k l. True}\<close>])
     unfolding linfun_cspan
-    using * apply (auto simp: cblinfun_apply_add clinearI
+    using * apply (auto simp: cblinfun.add_right clinearI
                         intro!: clinear_compose[unfolded o_def, where f=\<open>tensor_op a\<close> and g=\<open>(*\<^sub>V) G\<close>])
     apply (meson cbilinear_def tensor_op_cbilinear)
     using assms unfolding cbilinear_def by blast
@@ -253,7 +261,7 @@ proof -
   have \<open>clinear F2' \<and> (\<forall>a b. F2' (tensor_op a b) = F2 a b)\<close>
     unfolding F2'_def tensor_lift_def 
     apply (rule someI[where x=\<open>(*\<^sub>V) G\<close> and P=\<open>\<lambda>G. clinear G \<and> (\<forall>a b. G (tensor_op a b) = F2 a b)\<close>])
-    using G_F2 by (simp add: cblinfun_apply_add clinearI)
+    using G_F2 by (simp add: cblinfun.add_right clinearI)
 
   then show \<open>clinear F2'\<close> and \<open>(\<lambda>a b. tensor_lift F2 (tensor_op a b)) = F2\<close>
     unfolding F2'_def by auto
@@ -281,13 +289,13 @@ lift_definition assoc_ell2' :: \<open>('a::finite\<times>('b::finite\<times>'c::
 
 lemma assoc_ell2_tensor: \<open>assoc_ell2 *\<^sub>V tensor_ell2 (tensor_ell2 a b) c = tensor_ell2 a (tensor_ell2 b c)\<close>
   apply (rule clinear_equal_ket[THEN fun_cong, where x=a])
-    apply (simp add: cblinfun_apply_add clinearI tensor_ell2_add1 tensor_ell2_scaleC1)
+    apply (simp add: cblinfun.add_right clinearI tensor_ell2_add1 tensor_ell2_scaleC1)
    apply (simp add: clinear_tensor_ell22)
   apply (rule clinear_equal_ket[THEN fun_cong, where x=b])
-    apply (simp add: cblinfun_apply_add clinearI tensor_ell2_add1 tensor_ell2_add2 tensor_ell2_scaleC1 tensor_ell2_scaleC2)
+    apply (simp add: cblinfun.add_right clinearI tensor_ell2_add1 tensor_ell2_add2 tensor_ell2_scaleC1 tensor_ell2_scaleC2)
    apply (simp add: clinearI tensor_ell2_add1 tensor_ell2_add2 tensor_ell2_scaleC1 tensor_ell2_scaleC2)
   apply (rule clinear_equal_ket[THEN fun_cong, where x=c])
-    apply (simp add: cblinfun_apply_add clinearI tensor_ell2_add2 tensor_ell2_scaleC2)
+    apply (simp add: cblinfun.add_right clinearI tensor_ell2_add2 tensor_ell2_scaleC2)
    apply (simp add: clinearI tensor_ell2_add2 tensor_ell2_scaleC2)
   unfolding assoc_ell2.rep_eq
   apply transfer
@@ -295,28 +303,28 @@ lemma assoc_ell2_tensor: \<open>assoc_ell2 *\<^sub>V tensor_ell2 (tensor_ell2 a 
 
 lemma assoc_ell2'_tensor: \<open>assoc_ell2' *\<^sub>V tensor_ell2 a (tensor_ell2 b c) = tensor_ell2 (tensor_ell2 a b) c\<close>
   apply (rule clinear_equal_ket[THEN fun_cong, where x=a])
-    apply (simp add: cblinfun_apply_add clinearI tensor_ell2_add1 tensor_ell2_scaleC1)
+    apply (simp add: cblinfun.add_right clinearI tensor_ell2_add1 tensor_ell2_scaleC1)
    apply (simp add: clinearI tensor_ell2_add1 tensor_ell2_scaleC1)
   apply (rule clinear_equal_ket[THEN fun_cong, where x=b])
-    apply (simp add: cblinfun_apply_add clinearI tensor_ell2_add1 tensor_ell2_add2 tensor_ell2_scaleC1 tensor_ell2_scaleC2)
+    apply (simp add: cblinfun.add_right clinearI tensor_ell2_add1 tensor_ell2_add2 tensor_ell2_scaleC1 tensor_ell2_scaleC2)
    apply (simp add: clinearI tensor_ell2_add1 tensor_ell2_add2 tensor_ell2_scaleC1 tensor_ell2_scaleC2)
   apply (rule clinear_equal_ket[THEN fun_cong, where x=c])
-    apply (simp add: cblinfun_apply_add clinearI tensor_ell2_add2 tensor_ell2_scaleC2)
+    apply (simp add: cblinfun.add_right clinearI tensor_ell2_add2 tensor_ell2_scaleC2)
    apply (simp add: clinearI tensor_ell2_add2 tensor_ell2_scaleC2)
   unfolding assoc_ell2'.rep_eq
   apply transfer
   by auto
 
 lemma adjoint_assoc_ell2[simp]: \<open>assoc_ell2* = assoc_ell2'\<close>
-proof (rule adjoint_D[symmetric])
+proof (rule adjoint_eqI[symmetric])
   have [simp]: \<open>clinear (cinner (assoc_ell2' *\<^sub>V x))\<close> for x :: \<open>('a \<times> 'b \<times> 'c) ell2\<close>
-    by (metis (no_types, lifting) cblinfun_apply_add cinner_scaleC_right clinearI complex_scaleC_def mult.comm_neutral of_complex_def vector_to_cblinfun_adj_times_vec)
+    by (metis (no_types, lifting) cblinfun.add_right cinner_scaleC_right clinearI complex_scaleC_def mult.comm_neutral of_complex_def vector_to_cblinfun_adj_apply)
   have [simp]: \<open>clinear (\<lambda>a. \<langle>x, assoc_ell2 *\<^sub>V a\<rangle>)\<close> for x :: \<open>('a \<times> 'b \<times> 'c) ell2\<close>
-    by (simp add: cblinfun_apply_add cinner_add_right clinearI)
+    by (simp add: cblinfun.add_right cinner_add_right clinearI)
   have [simp]: \<open>antilinear (\<lambda>a. \<langle>a, y\<rangle>)\<close> for y :: \<open>('a \<times> 'b \<times> 'c) ell2\<close>
     using bounded_antilinear_cinner_left bounded_antilinear_def by blast
   have [simp]: \<open>antilinear (\<lambda>a. \<langle>assoc_ell2' *\<^sub>V a, y\<rangle>)\<close> for y :: \<open>(('a \<times> 'b) \<times> 'c) ell2\<close>
-    by (simp add: cblinfun_apply_add cinner_add_left antilinearI)
+    by (simp add: cblinfun.add_right cinner_add_left antilinearI)
   have \<open>\<langle>assoc_ell2' *\<^sub>V (ket x), ket y\<rangle> = \<langle>ket x, assoc_ell2 *\<^sub>V ket y\<rangle>\<close> for x :: \<open>'a \<times> 'b \<times> 'c\<close> and y
     apply (cases x, cases y)
     by (simp flip: tensor_ell2_ket add: assoc_ell2'_tensor assoc_ell2_tensor)
@@ -335,11 +343,11 @@ lemma tensor_ell2_extensionality:
   apply (rule equal_ket, case_tac x, hypsubst_thin)
   by (simp add: assms flip: tensor_ell2_ket)
 
-lemma assoc_ell2'_assoc_ell2[simp]: \<open>assoc_ell2' o\<^sub>C\<^sub>L assoc_ell2 = idOp\<close>
-  by (auto intro!: equal_ket simp: times_applyOp assoc_ell2'_tensor assoc_ell2_tensor simp flip: tensor_ell2_ket)
+lemma assoc_ell2'_assoc_ell2[simp]: \<open>assoc_ell2' o\<^sub>C\<^sub>L assoc_ell2 = id_cblinfun\<close>
+  by (auto intro!: equal_ket simp: cblinfun_apply_cblinfun_compose assoc_ell2'_tensor assoc_ell2_tensor simp flip: tensor_ell2_ket)
 
-lemma assoc_ell2_assoc_ell2'[simp]: \<open>assoc_ell2 o\<^sub>C\<^sub>L assoc_ell2' = idOp\<close>
-  by (auto intro!: equal_ket simp: times_applyOp assoc_ell2'_tensor assoc_ell2_tensor simp flip: tensor_ell2_ket)
+lemma assoc_ell2_assoc_ell2'[simp]: \<open>assoc_ell2 o\<^sub>C\<^sub>L assoc_ell2' = id_cblinfun\<close>
+  by (auto intro!: equal_ket simp: cblinfun_apply_cblinfun_compose assoc_ell2'_tensor assoc_ell2_tensor simp flip: tensor_ell2_ket)
 
 lemma unitary_assoc_ell2[simp]: "unitary assoc_ell2"
   unfolding unitary_def by auto
@@ -360,12 +368,12 @@ lemma tensor_op_right_add: \<open>b \<otimes>\<^sub>o (x + y) = b \<otimes>\<^su
 lemma tensor_op_scaleC_left: \<open>(c *\<^sub>C x) \<otimes>\<^sub>o b = c *\<^sub>C (x \<otimes>\<^sub>o b)\<close>
   for x :: \<open>'a::finite ell2 \<Rightarrow>\<^sub>C\<^sub>L 'c::finite ell2\<close> and b :: \<open>'b::finite ell2 \<Rightarrow>\<^sub>C\<^sub>L 'd::finite ell2\<close>
   apply (auto intro!: equal_ket simp: tensor_op_ket)
-  using tensor_ell2_scaleC1 by blast
+  by (metis scaleC_cblinfun.rep_eq tensor_ell2_ket tensor_ell2_scaleC1 tensor_op_ell2)
 
 lemma tensor_op_scaleC_right: \<open>b \<otimes>\<^sub>o (c *\<^sub>C x) = c *\<^sub>C (b \<otimes>\<^sub>o x)\<close>
   for x :: \<open>'a::finite ell2 \<Rightarrow>\<^sub>C\<^sub>L 'c::finite ell2\<close> and b :: \<open>'b::finite ell2 \<Rightarrow>\<^sub>C\<^sub>L 'd::finite ell2\<close>
   apply (auto intro!: equal_ket simp: tensor_op_ket)
-  by (simp add: tensor_ell2_scaleC2)
+  by (metis scaleC_cblinfun.rep_eq tensor_ell2_ket tensor_ell2_scaleC2 tensor_op_ell2)
 
 lemma clinear_tensor_left[simp]: \<open>clinear (\<lambda>a. a \<otimes>\<^sub>o b :: _::finite ell2 \<Rightarrow>\<^sub>C\<^sub>L _::finite ell2)\<close>
   apply (rule clinearI)
