Quantum_Extra.thy
@@ -20,9 +20,9 @@ lemma register_id'[simp]: \<open>register (\<lambda>x. x)\<close>
 
 lemma register_projector:
   assumes "register F"
-  assumes "isProjector a"
-  shows "isProjector (F a)"
-  using assms unfolding register_def isProjector_algebraic by metis
+  assumes "is_Proj a"
+  shows "is_Proj (F a)"
+  using assms unfolding register_def is_Proj_algebraic by metis
 
 lemma register_unitary:
   assumes "register F"
@@ -31,22 +31,22 @@ lemma register_unitary:
   using assms by (smt (verit, best) register_def unitary_def)
 
 lemma compatible_proj_intersect:
-  (* I think this also holds without isProjector, but my proof idea uses the Penrose-Moore 
+  (* I think this also holds without is_Proj, but my proof idea uses the Penrose-Moore 
      pseudoinverse or simultaneous diagonalization and we do not have an existence theorem for it. *)
-  assumes "compatible R S" and "isProjector a" and "isProjector b"
+  assumes "compatible R S" and "is_Proj a" and "is_Proj b"
   shows "(R a *\<^sub>S \<top>) \<sqinter> (S b *\<^sub>S \<top>) = ((R a o\<^sub>C\<^sub>L S b) *\<^sub>S \<top>)"
 proof (rule antisym)
   have "((R a o\<^sub>C\<^sub>L S b) *\<^sub>S \<top>) \<le> (S b *\<^sub>S \<top>)"
     apply (subst swap_registers[OF assms(1)])
-    by (auto simp: cblinfun_apply_assoc_subspace intro!: applyOpSpace_mono)
+    by (simp add: cblinfun_compose_image cblinfun_image_mono)
   moreover have "((R a o\<^sub>C\<^sub>L S b) *\<^sub>S \<top>) \<le> (R a *\<^sub>S \<top>)"
-    by (auto simp: cblinfun_apply_assoc_subspace intro!: applyOpSpace_mono)
+    by (simp add: cblinfun_compose_image cblinfun_image_mono)
   ultimately show \<open>((R a o\<^sub>C\<^sub>L S b) *\<^sub>S \<top>) \<le> (R a *\<^sub>S \<top>) \<sqinter> (S b *\<^sub>S \<top>)\<close>
     by auto
 
-  have "isProjector (R a)"
+  have "is_Proj (R a)"
     using assms(1) assms(2) compatible_register1 register_projector by blast
-  have "isProjector (S b)"
+  have "is_Proj (S b)"
     using assms(1) assms(3) compatible_register2 register_projector by blast
   show \<open>(R a *\<^sub>S \<top>) \<sqinter> (S b *\<^sub>S \<top>) \<le> (R a o\<^sub>C\<^sub>L S b) *\<^sub>S \<top>\<close>
   proof (unfold less_eq_ccsubspace.rep_eq, rule)
@@ -55,13 +55,13 @@ proof (rule antisym)
     then have \<open>\<psi> \<in> space_as_set (R a *\<^sub>S \<top>)\<close>
       by auto
     then have R: \<open>R a *\<^sub>V \<psi> = \<psi>\<close>
-      using \<open>isProjector (R a)\<close> apply_left_neutral isProjector_algebraic by blast
+      using \<open>is_Proj (R a)\<close> cblinfun_fixes_range is_Proj_algebraic by blast
     from asm have \<open>\<psi> \<in> space_as_set (S b *\<^sub>S \<top>)\<close>
       by auto
     then have S: \<open>S b *\<^sub>V \<psi> = \<psi>\<close>
-      using \<open>isProjector (S b)\<close> apply_left_neutral isProjector_algebraic by blast
+      using \<open>is_Proj (S b)\<close> cblinfun_fixes_range is_Proj_algebraic by blast
     from R S have \<open>\<psi> = (R a o\<^sub>C\<^sub>L S b) *\<^sub>V \<psi>\<close>
-      by (simp add: times_applyOp)
+      by (simp add: cblinfun_apply_cblinfun_compose)
     also have \<open>\<dots> \<in> space_as_set ((R a o\<^sub>C\<^sub>L S b) *\<^sub>S \<top>)\<close>
       apply simp by (metis R S calculation cblinfun_apply_in_image)
     finally show \<open>\<psi> \<in> space_as_set ((R a o\<^sub>C\<^sub>L S b) *\<^sub>S \<top>)\<close>
@@ -70,17 +70,20 @@ proof (rule antisym)
 qed
 
 lemma compatible_proj_mult:
-  assumes "compatible R S" and "isProjector a" and "isProjector b"
-  shows "isProjector (R a o\<^sub>C\<^sub>L S b)"
+  assumes "compatible R S" and "is_Proj a" and "is_Proj b"
+  shows "is_Proj (R a o\<^sub>C\<^sub>L S b)"
   using [[simproc del: Laws_Quantum.compatibility_warn]]
-  using assms unfolding isProjector_algebraic compatible_def
+  using assms unfolding is_Proj_algebraic compatible_def
   apply auto
-  apply (metis (no_types, lifting) cblinfun_apply_assoc register_mult)
-  by (simp add: assms(2) assms(3) isProjector_D2 register_projector)
+   apply (metis (no_types, lifting) cblinfun_compose_assoc register_mult)
+  by (simp add: assms(2) assms(3) is_proj_selfadj register_projector)
 
 lemma unitary_sandwich_register: \<open>unitary a \<Longrightarrow> register (sandwich a)\<close>
   unfolding register_def sandwich_def
-  by (smt (z3) adjoint_twice assoc_left(1) cblinfun_apply_dist1 cblinfun_apply_dist2 clinearI op_scalar_op scalar_op_op times_adjoint times_idOp2 unitary_def)
+  apply auto
+    apply (smt (verit) clinear_iff clinear_sandwich sandwich_def)
+   apply (metis (no_types, lifting) cblinfun_assoc_left(1) cblinfun_compose_id_right unitaryD1)
+  by (simp add: lift_cblinfun_comp(2))
 
 lemma sandwich_tensor: 
   fixes a :: \<open>'a::finite ell2 \<Rightarrow>\<^sub>C\<^sub>L 'a ell2\<close> and b :: \<open>'b::finite ell2 \<Rightarrow>\<^sub>C\<^sub>L 'b ell2\<close> 
@@ -92,7 +95,7 @@ lemma sandwich_tensor:
 lemma sandwich_grow_left: 
   fixes a :: \<open>'a::finite ell2 \<Rightarrow>\<^sub>C\<^sub>L 'a ell2\<close>
   assumes "unitary a"
-  shows "sandwich a \<otimes>\<^sub>r id = sandwich (a \<otimes>\<^sub>o idOp)"
+  shows "sandwich a \<otimes>\<^sub>r id = sandwich (a \<otimes>\<^sub>o id_cblinfun)"
   by (simp add: unitary_sandwich_register assms sandwich_tensor sandwich_id)
 
 lemma register_sandwich: \<open>register F \<Longrightarrow> F (sandwich a b) = sandwich (F a) (F b)\<close>
@@ -103,7 +106,7 @@ lemma assoc_ell2_sandwich: \<open>assoc = sandwich assoc_ell2\<close>
     apply (simp_all add: unitary_sandwich_register)[2]
   apply (rule equal_ket)
   apply (case_tac x)
-  by (simp add: sandwich_def assoc_apply times_applyOp tensor_op_ell2 assoc_ell2_tensor assoc_ell2'_tensor
+  by (simp add: sandwich_def assoc_apply cblinfun_apply_cblinfun_compose tensor_op_ell2 assoc_ell2_tensor assoc_ell2'_tensor
            flip: tensor_ell2_ket)
 
 lemma assoc_ell2'_sandwich: \<open>assoc' = sandwich assoc_ell2'\<close>
@@ -111,19 +114,19 @@ lemma assoc_ell2'_sandwich: \<open>assoc' = sandwich assoc_ell2'\<close>
     apply (simp_all add: unitary_sandwich_register)[2]
   apply (rule equal_ket)
   apply (case_tac x)
-  by (simp add: sandwich_def assoc'_apply times_applyOp tensor_op_ell2 assoc_ell2_tensor assoc_ell2'_tensor 
+  by (simp add: sandwich_def assoc'_apply cblinfun_apply_cblinfun_compose tensor_op_ell2 assoc_ell2_tensor assoc_ell2'_tensor 
            flip: tensor_ell2_ket)
 
 lemma swap_sandwich: "swap = sandwich Uswap"
   apply (rule tensor_extensionality)
     apply (auto simp: sandwich_def)[2]
   apply (rule tensor_ell2_extensionality)
-  by (simp add: sandwich_def times_applyOp tensor_op_ell2)
+  by (simp add: sandwich_def cblinfun_apply_cblinfun_compose tensor_op_ell2)
 
 lemma id_tensor_sandwich: 
   fixes a :: "'a::finite ell2 \<Rightarrow>\<^sub>C\<^sub>L 'b::finite ell2"
   assumes "unitary a"
-  shows "id \<otimes>\<^sub>r sandwich a = sandwich (idOp \<otimes>\<^sub>o a)"
+  shows "id \<otimes>\<^sub>r sandwich a = sandwich (id_cblinfun \<otimes>\<^sub>o a)"
   apply (rule tensor_extensionality) 
   using assms by (auto simp: register_tensor_is_hom comp_tensor_op sandwich_def tensor_op_adjoint unitary_sandwich_register)
 
@@ -134,7 +137,7 @@ lemma compatible_selfbutter_join:
   using assms by auto
 
 definition empty_var :: \<open>'a::{CARD_1,enum} update \<Rightarrow> 'b::finite update\<close> where
-  "empty_var a = one_dim_iso a *\<^sub>C idOp"
+  "empty_var a = one_dim_iso a *\<^sub>C id_cblinfun"
 
 lemma register_empty_var[simp]: \<open>register empty_var\<close>
   unfolding register_def empty_var_def
