Teleport.thy
@@ -42,48 +42,48 @@ definition "teleport a b = [
     apply hadamard X,
     ifthen \<Phi>1 a,
     ifthen X b, 
-    apply (if a=1 then pauliX else idOp) \<Phi>2,
-    apply (if b=1 then pauliZ else idOp) \<Phi>2
+    apply (if a=1 then pauliX else id_cblinfun) \<Phi>2,
+    apply (if b=1 then pauliZ else id_cblinfun) \<Phi>2
   ]"
 
 
-lemma \<Phi>_X\<Phi>: \<open>\<Phi> a = X\<Phi> (idOp \<otimes>\<^sub>o a)\<close>
+lemma \<Phi>_X\<Phi>: \<open>\<Phi> a = X\<Phi> (id_cblinfun \<otimes>\<^sub>o a)\<close>
   by (auto simp: register_pair_apply)
-lemma X\<Phi>1_X\<Phi>: \<open>X\<Phi>1 a = X\<Phi> (assoc (a \<otimes>\<^sub>o idOp))\<close>
+lemma X\<Phi>1_X\<Phi>: \<open>X\<Phi>1 a = X\<Phi> (assoc (a \<otimes>\<^sub>o id_cblinfun))\<close>
   apply (subst pair_o_assoc[unfolded o_def, of X \<Phi>1 \<Phi>2, simplified, THEN fun_cong])
   by (auto simp: register_pair_apply)
-lemma X\<Phi>2_X\<Phi>: \<open>X\<Phi>2 a = X\<Phi> ((id \<otimes>\<^sub>r swap) (assoc (a \<otimes>\<^sub>o idOp)))\<close>
+lemma X\<Phi>2_X\<Phi>: \<open>X\<Phi>2 a = X\<Phi> ((id \<otimes>\<^sub>r swap) (assoc (a \<otimes>\<^sub>o id_cblinfun)))\<close>
   apply (subst pair_o_tensor[unfolded o_def, THEN fun_cong], simp, simp, simp)
   apply (subst (2) register_Fst_register_Snd[symmetric, of \<Phi>], simp)
   using [[simproc del: compatibility_warn]]
   apply (subst pair_o_swap[unfolded o_def], simp)
   apply (subst pair_o_assoc[unfolded o_def, THEN fun_cong], simp, simp, simp)
   by (auto simp: register_pair_apply)
-lemma \<Phi>2_X\<Phi>: \<open>\<Phi>2 a = X\<Phi> (idOp \<otimes>\<^sub>o (idOp \<otimes>\<^sub>o a))\<close>
+lemma \<Phi>2_X\<Phi>: \<open>\<Phi>2 a = X\<Phi> (id_cblinfun \<otimes>\<^sub>o (id_cblinfun \<otimes>\<^sub>o a))\<close>
   by (auto simp: Snd_def register_pair_apply)
-lemma X_X\<Phi>: \<open>X a = X\<Phi> (a \<otimes>\<^sub>o idOp)\<close>
+lemma X_X\<Phi>: \<open>X a = X\<Phi> (a \<otimes>\<^sub>o id_cblinfun)\<close>
   by (auto simp: register_pair_apply)
-lemma \<Phi>1_X\<Phi>: \<open>\<Phi>1 a = X\<Phi> (idOp \<otimes>\<^sub>o (a \<otimes>\<^sub>o idOp))\<close>
+lemma \<Phi>1_X\<Phi>: \<open>\<Phi>1 a = X\<Phi> (id_cblinfun \<otimes>\<^sub>o (a \<otimes>\<^sub>o id_cblinfun))\<close>
   by (auto simp: Fst_def register_pair_apply)
 lemmas to_X\<Phi> = \<Phi>_X\<Phi> X\<Phi>1_X\<Phi> X\<Phi>2_X\<Phi> \<Phi>2_X\<Phi> X_X\<Phi> \<Phi>1_X\<Phi>
 
-lemma X_X\<Phi>1: \<open>X a = X\<Phi>1 (a \<otimes>\<^sub>o idOp)\<close>
+lemma X_X\<Phi>1: \<open>X a = X\<Phi>1 (a \<otimes>\<^sub>o id_cblinfun)\<close>
   by (auto simp: register_pair_apply)
 lemmas to_X\<Phi>1 = X_X\<Phi>1
 
-lemma XAB_to_X\<Phi>2_AB: \<open>XAB a = (X\<Phi>2;AB) ((swap \<otimes>\<^sub>r id) (assoc' (idOp \<otimes>\<^sub>o assoc a)))\<close>
+lemma XAB_to_X\<Phi>2_AB: \<open>XAB a = (X\<Phi>2;AB) ((swap \<otimes>\<^sub>r id) (assoc' (id_cblinfun \<otimes>\<^sub>o assoc a)))\<close>
   by (simp add: pair_o_tensor[unfolded o_def, THEN fun_cong] register_pair_apply
       pair_o_swap[unfolded o_def, THEN fun_cong]
       pair_o_assoc'[unfolded o_def, THEN fun_cong]
       pair_o_assoc[unfolded o_def, THEN fun_cong])
 
-lemma X\<Phi>2_to_X\<Phi>2_AB: \<open>X\<Phi>2 a = (X\<Phi>2;AB) (a \<otimes>\<^sub>o idOp)\<close>
+lemma X\<Phi>2_to_X\<Phi>2_AB: \<open>X\<Phi>2 a = (X\<Phi>2;AB) (a \<otimes>\<^sub>o id_cblinfun)\<close>
   by (simp add: register_pair_apply)
 
 schematic_goal \<Phi>2AB_to_X\<Phi>2_AB: "\<Phi>2AB a = (X\<Phi>2;AB) ?b"
   apply (subst pair_o_assoc'[unfolded o_def, THEN fun_cong])
      apply simp_all[3]
-  apply (subst register_pair_apply[where a=idOp])
+  apply (subst register_pair_apply[where a=id_cblinfun])
     apply simp_all[2]
   apply (subst pair_o_assoc[unfolded o_def, THEN fun_cong])
      apply simp_all[3]
@@ -95,7 +95,7 @@ lemma teleport:
   assumes [simp]: "norm \<psi> = 1"
   shows "hoare (XAB =\<^sub>q \<psi> \<sqinter> \<Phi> =\<^sub>q \<beta>00) (teleport a b) (\<Phi>2AB =\<^sub>q \<psi>)"
 proof -
-  define XZ :: \<open>bit update\<close> where "XZ = (if a=1 then (if b=1 then pauliZ o\<^sub>C\<^sub>L pauliX else pauliX) else (if b=1 then pauliZ else idOp))"
+  define XZ :: \<open>bit update\<close> where "XZ = (if a=1 then (if b=1 then pauliZ o\<^sub>C\<^sub>L pauliX else pauliX) else (if b=1 then pauliZ else id_cblinfun))"
 
   define pre where "pre = XAB =\<^sub>q \<psi>"
 
@@ -103,42 +103,42 @@ proof -
   have \<open>(XAB =\<^sub>q \<psi> \<sqinter> \<Phi> =\<^sub>q \<beta>00) = O1 *\<^sub>S pre\<close>
     unfolding pre_def O1_def EQ_def
     apply (subst compatible_proj_intersect[where R=XAB and S=\<Phi>])
-       apply (simp_all add: butterfly_isProjector)
+       apply (simp_all add: butterfly_is_Proj)
     apply (subst swap_registers[where R=XAB and S=\<Phi>])
-    by (simp_all add: assoc_left(2))
+    by (simp_all add: cblinfun_assoc_left(2))
 
   also
   define O2 where "O2 = X\<Phi>1 CNOT o\<^sub>C\<^sub>L O1"
   have \<open>hoare (O1 *\<^sub>S pre) [apply CNOT X\<Phi>1] (O2 *\<^sub>S pre)\<close>
-    apply (rule hoare_apply) by (simp add: O2_def assoc_left(2))
+    apply (rule hoare_apply) by (simp add: O2_def cblinfun_assoc_left(2))
 
   also
   define O3 where \<open>O3 = X hadamard o\<^sub>C\<^sub>L O2\<close>
   have \<open>hoare (O2 *\<^sub>S pre) [apply hadamard X] (O3 *\<^sub>S pre)\<close>
-    apply (rule hoare_apply) by (simp add: O3_def assoc_left(2))
+    apply (rule hoare_apply) by (simp add: O3_def cblinfun_assoc_left(2))
 
   also
   define O4 where \<open>O4 = \<Phi>1 (selfbutterket a) o\<^sub>C\<^sub>L O3\<close>
   have \<open>hoare (O3 *\<^sub>S pre) [ifthen \<Phi>1 a] (O4 *\<^sub>S pre)\<close>
-    apply (rule hoare_ifthen) by (simp add: O4_def assoc_left(2))
+    apply (rule hoare_ifthen) by (simp add: O4_def cblinfun_assoc_left(2))
 
   also
   define O5 where \<open>O5 = X (selfbutterket b) o\<^sub>C\<^sub>L O4\<close>
   have \<open>hoare (O4 *\<^sub>S pre) [ifthen X b] (O5 *\<^sub>S pre)\<close>
-    apply (rule hoare_ifthen) by (simp add: O5_def assoc_left(2))
+    apply (rule hoare_ifthen) by (simp add: O5_def cblinfun_assoc_left(2))
 
   also
-  define O6 where \<open>O6 = \<Phi>2 (if a=1 then pauliX else idOp) o\<^sub>C\<^sub>L O5\<close>
-  have \<open>hoare (O5 *\<^sub>S pre) [apply (if a=1 then pauliX else idOp) (\<Phi> \<circ> Snd)] (O6 *\<^sub>S pre)\<close>
-    apply (rule hoare_apply) by (auto simp add: O6_def assoc_left(2))
+  define O6 where \<open>O6 = \<Phi>2 (if a=1 then pauliX else id_cblinfun) o\<^sub>C\<^sub>L O5\<close>
+  have \<open>hoare (O5 *\<^sub>S pre) [apply (if a=1 then pauliX else id_cblinfun) (\<Phi> \<circ> Snd)] (O6 *\<^sub>S pre)\<close>
+    apply (rule hoare_apply) by (auto simp add: O6_def cblinfun_assoc_left(2))
 
   also
-  define O7 where \<open>O7 = \<Phi>2 (if b = 1 then pauliZ else idOp) o\<^sub>C\<^sub>L O6\<close>
+  define O7 where \<open>O7 = \<Phi>2 (if b = 1 then pauliZ else id_cblinfun) o\<^sub>C\<^sub>L O6\<close>
   have O7: \<open>O7 = \<Phi>2 XZ o\<^sub>C\<^sub>L O5\<close>
     by (auto simp add: O6_def O7_def XZ_def register_mult lift_cblinfun_comp[OF register_mult])
-  have \<open>hoare (O6 *\<^sub>S pre) [apply (if b=1 then pauliZ else idOp) (\<Phi> \<circ> Snd)] (O7 *\<^sub>S pre)\<close>
+  have \<open>hoare (O6 *\<^sub>S pre) [apply (if b=1 then pauliZ else id_cblinfun) (\<Phi> \<circ> Snd)] (O7 *\<^sub>S pre)\<close>
     apply (rule hoare_apply) 
-    by (auto simp add: O7_def assoc_left(2))
+    by (auto simp add: O7_def cblinfun_assoc_left(2))
 
   finally have hoare: \<open>hoare (XAB =\<^sub>q \<psi> \<sqinter> \<Phi> =\<^sub>q \<beta>00) (teleport a b) (O7 *\<^sub>S pre)\<close>
     by (auto simp add: teleport_def comp_def)
@@ -152,7 +152,7 @@ proof -
     apply (rule arg_cong[of _ _ X\<Phi>])
     apply (rule cblinfun_eq_mat_of_cblinfunI)
     apply (simp add: assoc_ell2_sandwich mat_of_cblinfun_tensor_op XZ_def
-                     butterfly_def' cblinfun_of_mat_timesOp mat_of_cblinfun_ell2_to_l2bounded 
+                     butterfly_def cblinfun_of_mat_timesOp mat_of_cblinfun_ell2_to_l2bounded 
                      mat_of_cblinfun_adjoint' vec_of_onb_enum_ket 
                      cblinfun_of_mat_id swap_sandwich[abs_def] mat_of_cblinfun_scaleR mat_of_cblinfun_scalarMult
                      id_tensor_sandwich vec_of_onb_enum_tensor_state mat_of_cblinfun_description
@@ -161,28 +161,28 @@ proof -
 
   have [simp]: "unitary XZ"
     unfolding unitary_def unfolding XZ_def apply auto
-    apply (metis assoc_left(1) pauliXX pauliZZ times_idOp2)
-    by (metis assoc_left(1) pauliXX pauliZZ times_idOp2)
+    apply (metis cblinfun_assoc_left(1) pauliXX pauliZZ cblinfun_compose_id_left)
+    by (metis cblinfun_assoc_left(1) pauliXX pauliZZ cblinfun_compose_id_left)
 
   have O7': "O7 = (1/2) *\<^sub>C X\<Phi>2 Uswap o\<^sub>C\<^sub>L \<Phi> (butterfly (ket a \<otimes>\<^sub>s ket b) \<beta>00)"
     unfolding O7 O5'
-    by (simp add: cblinfun_apply_assoc[symmetric] register_mult[of \<Phi>2] del: comp_apply)
+    by (simp add: cblinfun_compose_assoc[symmetric] register_mult[of \<Phi>2] del: comp_apply)
 
   have "O7 *\<^sub>S pre = X\<Phi>2 Uswap *\<^sub>S XAB (selfbutter \<psi>) *\<^sub>S \<Phi> (butterfly (ket (a, b)) \<beta>00) *\<^sub>S \<top>"
-    apply (simp add: O7' pre_def EQ_def cblinfun_apply_assoc_subspace)
+    apply (simp add: O7' pre_def EQ_def cblinfun_compose_image)
     apply (subst lift_cblinfun_comp[OF swap_registers[where R=\<Phi> and S=XAB]], simp)
-    by (simp add: assoc_left(2))
+    by (simp add: cblinfun_assoc_left(2))
   also have \<open>\<dots> \<le> X\<Phi>2 Uswap *\<^sub>S XAB (selfbutter \<psi>) *\<^sub>S \<top>\<close>
-    by (simp add: applyOpSpace_mono)
-  also have \<open>\<dots> = (X\<Phi>2;AB) (Uswap \<otimes>\<^sub>o idOp) *\<^sub>S (X\<Phi>2;AB)
-                      ((swap \<otimes>\<^sub>r id) (assoc' (idOp \<otimes>\<^sub>o assoc (selfbutter \<psi>)))) *\<^sub>S \<top>\<close>
+    by (simp add: cblinfun_image_mono)
+  also have \<open>\<dots> = (X\<Phi>2;AB) (Uswap \<otimes>\<^sub>o id_cblinfun) *\<^sub>S (X\<Phi>2;AB)
+                      ((swap \<otimes>\<^sub>r id) (assoc' (id_cblinfun \<otimes>\<^sub>o assoc (selfbutter \<psi>)))) *\<^sub>S \<top>\<close>
     by (simp add: to_X\<Phi>2_AB)
   also have \<open>\<dots> = \<Phi>2AB (selfbutter \<psi>) *\<^sub>S X\<Phi>2 Uswap *\<^sub>S \<top>\<close>
     apply (simp add: swap_sandwich sandwich_grow_left to_X\<Phi>2_AB   
-        cblinfun_apply_assoc_subspace[symmetric] register_mult)
-    by (simp add: sandwich_def cblinfun_apply_assoc[symmetric] comp_tensor_op tensor_op_adjoint)
+        cblinfun_compose_image[symmetric] register_mult)
+    by (simp add: sandwich_def cblinfun_compose_assoc[symmetric] comp_tensor_op tensor_op_adjoint)
   also have \<open>\<dots> \<le> \<Phi>2AB =\<^sub>q \<psi>\<close>
-    by (simp add: EQ_def applyOpSpace_mono)
+    by (simp add: EQ_def cblinfun_image_mono)
   finally have \<open>O7 *\<^sub>S pre \<le> \<Phi>2AB =\<^sub>q \<psi>\<close>
     by simp
 
@@ -201,11 +201,11 @@ type_synonym b_state = "1000000 word"
 type_synonym mem = "a_state * bit * bit * b_state * bit"
 type_synonym 'a var = \<open>'a update \<Rightarrow> mem update\<close>
 
-definition A :: "a_state var" where \<open>A a = a \<otimes>\<^sub>o idOp \<otimes>\<^sub>o idOp \<otimes>\<^sub>o idOp \<otimes>\<^sub>o idOp\<close>
-definition X :: \<open>bit var\<close> where \<open>X a = idOp \<otimes>\<^sub>o a \<otimes>\<^sub>o idOp \<otimes>\<^sub>o idOp \<otimes>\<^sub>o idOp\<close>
-definition \<Phi>1 :: \<open>bit var\<close> where \<open>\<Phi>1 a = idOp \<otimes>\<^sub>o idOp \<otimes>\<^sub>o a \<otimes>\<^sub>o idOp \<otimes>\<^sub>o idOp\<close>
-definition B :: \<open>b_state var\<close> where \<open>B a = idOp \<otimes>\<^sub>o idOp \<otimes>\<^sub>o idOp \<otimes>\<^sub>o a \<otimes>\<^sub>o idOp\<close>
-definition \<Phi>2 :: \<open>bit var\<close> where \<open>\<Phi>2 a = idOp \<otimes>\<^sub>o idOp \<otimes>\<^sub>o idOp \<otimes>\<^sub>o idOp \<otimes>\<^sub>o a\<close>
+definition A :: "a_state var" where \<open>A a = a \<otimes>\<^sub>o id_cblinfun \<otimes>\<^sub>o id_cblinfun \<otimes>\<^sub>o id_cblinfun \<otimes>\<^sub>o id_cblinfun\<close>
+definition X :: \<open>bit var\<close> where \<open>X a = id_cblinfun \<otimes>\<^sub>o a \<otimes>\<^sub>o id_cblinfun \<otimes>\<^sub>o id_cblinfun \<otimes>\<^sub>o id_cblinfun\<close>
+definition \<Phi>1 :: \<open>bit var\<close> where \<open>\<Phi>1 a = id_cblinfun \<otimes>\<^sub>o id_cblinfun \<otimes>\<^sub>o a \<otimes>\<^sub>o id_cblinfun \<otimes>\<^sub>o id_cblinfun\<close>
+definition B :: \<open>b_state var\<close> where \<open>B a = id_cblinfun \<otimes>\<^sub>o id_cblinfun \<otimes>\<^sub>o id_cblinfun \<otimes>\<^sub>o a \<otimes>\<^sub>o id_cblinfun\<close>
+definition \<Phi>2 :: \<open>bit var\<close> where \<open>\<Phi>2 a = id_cblinfun \<otimes>\<^sub>o id_cblinfun \<otimes>\<^sub>o id_cblinfun \<otimes>\<^sub>o id_cblinfun \<otimes>\<^sub>o a\<close>
 
 end
 
